clight_examples/xorlist/xorlist01addproof.v
@@ -132,19 +132,15 @@ Section PROOF.
     iPoseProof ((@offset_cast_ptr _ _ _ _ Es) with "new_ofs") as "%".
     rewrite H4. rename H4 into new_cast_ptr.
     hred_r. unhide. remove_tau. unhide.
-    remove_tau. 
+    remove_tau.
 
     unfold full_xorlist.
     iDestruct "PRE" 
-      as (m_hd_hdl m_tl_hdl m_hd m_tl p_hd p_tl 
-          i_hd i_tl ofs_hd_hdl ofs_tl_hdl) "PRE".
+      as (m_hd_hdl m_tl_hdl hd tl ofs_hd_hdl ofs_tl_hdl) "PRE".
     iDestruct "PRE" as (tg_hd_hdl tg_tl_hdl) 
-      "[[[[[[[[[[hd_hdl_point hd_hdl_ofs] %] hd_addr] %]
-               tl_hdl_point] tl_hdl_ofs] %] tl_addr] %] LIST]".
+      "[[[[[[hd_hdl_point hd_hdl_ofs] %] tl_hdl_point] tl_hdl_ofs] %] LIST]".
     rename H4 into hd_hdl_align.
-    rename H5 into hd_null_case.
-    rename H6 into tl_hdl_align.
-    rename H7 into tl_null_case.
+    rename H5 into tl_hdl_align.
 
     iPoseProof (points_to_is_ptr with "hd_hdl_point") as "%".
     rewrite H4. rename H4 into hd_hdl_is_point. hred_r.
@@ -153,7 +149,8 @@ Section PROOF.
     iSplitL "INV hd_hdl_point hd_hdl_ofs"; iFrame.
     { rewrite encode_val_length. et. }
     iIntros (st_src1 st_tgt1) "[INV [hd_hdl_point hd_hdl_ofs]]".
-    replace (decode_val Mptr (encode_val Mptr p_hd)) with p_hd by admit "captured is decode_encode".
+    unfold Mptr. rewrite ptr64.
+    replace (decode_val Mint64 (encode_val Mint64 hd)) with hd by admit "fullxor's head is pointer".
 
     hred_r. unhide. remove_tau. unhide. remove_tau.
     iPoseProof (points_to_is_ptr with "tl_hdl_point") as "%".
@@ -163,7 +160,8 @@ Section PROOF.
     iSplitL "INV tl_hdl_point tl_hdl_ofs"; iFrame.
     { rewrite encode_val_length. et. }
     iIntros (st_src2 st_tgt2) "[INV [tl_hdl_point tl_hdl_ofs]]".
-    replace (decode_val Mptr (encode_val Mptr p_tl)) with p_tl by admit "captured is decode_encode".
+    unfold Mptr. rewrite ptr64. 
+    replace (decode_val Mint64 (encode_val Mint64 tl)) with tl by admit "fullxor's head is pointer".
 
     hred_r. unhide. remove_tau. unhide. remove_tau.
     iPoseProof (points_to_is_ptr with "new_point") as "%".
@@ -191,9 +189,10 @@ Section PROOF.
 
     destruct lfull.
     (* case: nil list *)
-    - unfold frag_xorlist at 1.
-      iDestruct "LIST" as "%". des. clarify.
-      hexploit hd_null_case; et. i. clarify.
+    - admit "".
+      (* unfold frag_xorlist at 1.
+      iDestruct "LIST" as "[end_equiv %]". des. clarify.
+      replace (Vptrofs Ptrofs.zero) with Vnullptr by et.
 
       iApply isim_ccallU_cmp_ptr0; ss; oauto.
       iSplitL "INV"; iFrame.
@@ -222,16 +221,9 @@ Section PROOF.
       replace (Ptrofs.add (Ptrofs.add _ _) _) with Ptrofs.zero.
       2:{ rewrite Ptrofs.add_assoc. ss. }
 
-      rewrite new_cast_ptr. hred_r. unhide.
-
-      iApply isim_ccallU_capture2; ss; oauto.
-      iSplitL "INV new_ofs"; try solve [iFrame].
-      iIntros (st_src6 st_tgt6 i) "[INV [new_ofs new_addr]]".
-
-      hred_r. unhide. remove_tau.
-      rewrite cast_ptrofs. hred_r. unhide. remove_tau.
+      rewrite new_cast_ptr. hred_r. unhide. remove_tau.
       rewrite tl_hdl_is_point. hred_r.
-      rewrite cast_ptrofs. hred_r.
+      rewrite new_cast_ptr. hred_r.
 
       iApply isim_ccallU_store; ss; oauto.
       iSplitL "INV tl_hdl_point tl_hdl_ofs"; iFrame.
@@ -240,7 +232,7 @@ Section PROOF.
 
       hred_r. unhide. remove_tau.
       rewrite hd_hdl_is_point. hred_r.
-      rewrite cast_ptrofs. hred_r.
+      rewrite new_cast_ptr. hred_r.
 
       iApply isim_ccallU_store; ss; oauto.
       iSplitL "INV hd_hdl_point hd_hdl_ofs"; iFrame.
@@ -252,9 +244,10 @@ Section PROOF.
       iExists _. iApply isim_ret.
       iFrame. iSplit; ss. iSplit; ss.
       replace (Vptrofs (Ptrofs.repr 8))
-        with (Vptrofs (Ptrofs.repr (length (encode_val Mptr (Vptrofs i))))) by ss.
+        with (Vptrofs (Ptrofs.repr (length (encode_val Mint64 (Vlong item))))) by ss.
       iCombine "new_point_item new_point_key" as "new_point".
       iPoseProof (points_to_collect with "new_point") as "new_point".
+      (* iPoseProof (points_to_collect with "new_point") as "new_point".
       iPoseProof (capture_dup with "new_addr") as "[new_addr new_addr']".
       iPoseProof (capture_dup with "new_addr'") as "[new_addr' new_addr'']".
       iPoseProof (capture_offset_comm with "new_addr'") as "comm".
@@ -262,21 +255,355 @@ Section PROOF.
       iPoseProof ("comm" with "new_ofs") as "new_ofs".
       iPoseProof ("comm'" with "new_point") as "new_point".
       iPoseProof (capture_refl with "new_addr") as "new_addr".
-      iPoseProof (capture_dup with "new_addr") as "[new_addr new_addr']".
-      iExists _,_,_,_,_,_,_,_. iExists _,_,_,_. iFrame.
+      iPoseProof (capture_dup with "new_addr") as "[new_addr new_addr']". *)
+      iExists _,_,_,_,_,_,_,_. iFrame.
       iSplit.
-      { iPureIntro. splits; ss. all: i; clarify. }
+      { iPureIntro. splits; ss. }
       unfold vlist_add.
       destruct (Val.eq _ _); ss.
-      + iExists _,_. iSplit; ss.
-        replace (Ptrofs.xor Ptrofs.zero Ptrofs.zero) with Ptrofs.zero by ss.
+      + iExists Ptrofs.zero,Ptrofs.zero,_,_.
+        replace (Ptrofs.xor _ _) with Ptrofs.zero by et.
         replace (Vptrofs Ptrofs.zero) with Vnullptr by et.
-        iFrame. ss.
-      + iExists _,_. iSplit; ss.
-        replace (Ptrofs.xor Ptrofs.zero Ptrofs.zero) with Ptrofs.zero by ss.
+        iFrame. instantiate (1:=m_new).
+        iSplitL.
+        { iSplit; ss. Transparent captured_to. unfold captured_to. des_ifs.
+          Opaque captured_to. }
+        { iSplit; ss. iLeft. ss. }
+      + iExists Ptrofs.zero,Ptrofs.zero,_,_.
+        replace (Ptrofs.xor _ _) with Ptrofs.zero by et.
         replace (Vptrofs Ptrofs.zero) with Vnullptr by et.
-        iFrame. ss.
-    - 
+        iFrame. instantiate (1:=m_new).
+        iSplitL.
+        { iSplit; ss. Transparent captured_to. unfold captured_to. des_ifs.
+          Opaque captured_to. }
+        { iSplit; ss. iLeft. ss. } *)
+    - ss. destruct v; try solve [iDestruct "LIST" as "%"; clarify].
+      iDestruct "LIST" as (i_prev i_next m_prev m_hd) 
+        "[[[[% prev_addr] hd_ofs] hd_point] LIST]".
+
+      iApply isim_ccallU_cmp_ptr3; ss; oauto.
+      iSplitL "INV hd_ofs".
+      { iFrame. iPureIntro. red. rewrite H4. ss. }
+      iIntros (st_src4 st_tgt4) "[INV hd_ofs]".
+
+      hred_r. des_ifs_safe. unhide. remove_tau.
+      des_ifs; cycle 1.
+      (* not nil, head case *)
+      + rename Heq0 into ISHEAD.
+        unhide. hred_r. unhide. remove_tau. unhide. remove_tau.
+        hexploit SKINCLENV.
+        { instantiate (2:="encrypt"). ss. }
+        i. des. ss. rewrite FIND. rename FIND into encrypt_loc.
+        hred_r. rewrite cast_long; et. hred_r. des_ifs. clear e.
+        rename H4 into m_hd_size.
+        iPoseProof ((@offset_cast_ptr _ _ _ _ Es) with "hd_ofs") as "%".
+        rewrite H4. hred_r.
+        rename H4 into hd_cast_ptr.
+
+        replace (pred _) with blk0 by nia.
+        erewrite SKINCLGD; et.
+        hred_r. ss.
+        replace (Vlong (Int64.repr _)) with Vnullptr by et.
+
+        iApply isim_ccallU_pure; et.
+        { eapply fn_has_spec_in_stb; et.
+          { eapply STBINCL. stb_tac. unfold xorStb.
+            unseal "stb". ss. }
+          { ss. instantiate (1:=inr (inr (inl (_,_,_,_,_)))).
+            ss. oauto. }
+          { ss. } }
+        { instantiate (1:=14). oauto. }
+        
+        ss. iSplitL "INV hd_ofs".
+        { iFrame. ss. }
+        iIntros (st_src5 st_tgt5 ret_src ret_tgt) "[INV [POST %]]".
+        iDestruct "POST" as (i_hd') "[[% hd_addr] hd_ofs]".
+        iExists _. iSplit; ss. clear H4 H5 Heq.
+
+        hred_r. unhide. remove_tau.
+        rewrite new_is_point. hred_r.
+        rewrite new_is_point. hred_r.
+        rewrite co_co_members. ss. hred_r.
+        replace (Coqlib.align _ _) with 8%Z by et.
+        rewrite cast_ptrofs. hred_r.
+
+        iApply isim_ccallU_store; ss; oauto.
+        iSplitL "INV new_point_key new_ofs".
+        { iFrame. iExists _. iFrame. iSplit.
+          2:{ iApply offset_slide. ss. }
+          iPureIntro. split; ss. exists 1. ss. }
+        iIntros (st_src6 st_tgt6) "[INV [new_point_key new_ofs]]".
+
+        hred_r. unhide. remove_tau. unhide. hred_r. unhide. remove_tau.
+        hexploit SKINCLENV.
+        { instantiate (2:="decrypt"). ss. }
+        i. des. ss. rewrite FIND. rename FIND into decrypt_loc.
+        hred_r.
+        iPoseProof (points_to_is_ptr with "hd_point") as "%".
+        rewrite H4. rename H4 into hd_is_point.
+        hred_r. rewrite hd_is_point. hred_r.
+        rewrite co_co_members. ss. hred_r.
+        replace (Coqlib.align _ _) with 8%Z by et.
+
+        iPoseProof (points_to_split with "hd_point") as "[hd_point_item hd_point_key]".
+        iApply isim_ccallU_load; ss; oauto.
+        iSplitL "INV hd_point_key hd_ofs".
+        { iFrame. iSplit.
+          { iApply offset_slide. ss. }
+          iPureIntro. rewrite encode_val_length.
+          split; ss. exists 1. ss. }
+        iIntros (st_src7 st_tgt7) "[INV [hd_point_key hd_ofs]]".
+
+        unfold Mptr. rewrite ptr64.
+        rewrite decode_encode_ofs. hred_r.
+        rewrite cast_long; et. hred_r.
+        rewrite cast_ptrofs. hred_r.
+        des_ifs_safe. clear e.
+
+        replace (pred _) with blk1 by nia.
+        erewrite SKINCLGD; et.
+        hred_r. ss.
+        replace (Vlong (Int64.repr _)) with Vnullptr by et.
+        iApply isim_ccallU_pure; et.
+        { eapply fn_has_spec_in_stb; et.
+          { eapply STBINCL. stb_tac. unfold xorStb.
+            unseal "stb". ss. }
+          { ss. instantiate (1:=(inr _)).
+            ss. oauto. }
+          { ss. } }
+        { instantiate (1:=11). oauto. }
+
+        ss. iSplitL "INV".
+        { iFrame. ss. }
+        iIntros (st_src8 st_tgt8 ret_src0 ret_tgt0) "[INV [POST %]]".
+        iDestruct "POST" as "%". clarify.
+        iExists _. iSplit; ss.
+
+        hred_r. unhide. remove_tau. unhide. hred_r. unhide. remove_tau.
+        unhide. remove_tau.
+        rewrite encrypt_loc. hred_r.
+        rewrite cast_ptrofs. hred_r.
+        rewrite new_cast_ptr. hred_r.
+        des_ifs. clear e. hred_r.
+        replace (pred _) with blk0 by nia.
+        erewrite SKINCLGD; et.
+        hred_r. ss.
+        replace i_prev with Ptrofs.zero by admit "vnullptr capture is zero".
+        rewrite Ptrofs.xor_zero_l.
+        destruct lfull; ss.
+        * iDestruct "LIST" as "[end_equiv %]". des. clarify.
+          replace i_next with Ptrofs.zero by admit "intval is equal".
+          replace (Vptrofs Ptrofs.zero) with Vnullptr by et.
+          iPoseProof ((offset_slide _ _ _ _ _ (Ptrofs.repr (-8)%Z)) with "new_ofs") as "new_ofs".
+          replace (Val.addl (Val.addl _ _) _) with p_new.
+          2:{ rewrite Val.addl_assoc. ss. }
+          replace (Ptrofs.add (Ptrofs.add _ _) _) with Ptrofs.zero.
+          2:{ rewrite Ptrofs.add_assoc. ss. }
+
+          iApply isim_ccallU_pure; et.
+          { eapply fn_has_spec_in_stb; et.
+            { eapply STBINCL. stb_tac. unfold xorStb.
+              unseal "stb". ss. }
+            { ss. instantiate (1:=(inr (inl (_,_,_,_,_)))).
+              ss. oauto. }
+            { ss. } }
+          { instantiate (1:=10). oauto. }
+
+          ss. iSplitL "INV new_ofs".
+          { iFrame. iPureIntro. ss. }
+          iIntros (st_src9 st_tgt9 ret_src0 ret_tgt0) "[INV [POST %]]".
+          iDestruct "POST" as (i_l) "[[% new_addr] new_ofs]".
+          rewrite H6. clear H6 H4.
+          iExists _. iSplit; ss.
+
+          hred_r. unhide. remove_tau.
+
+          iPoseProof (points_to_is_ptr with "hd_point_item") as "%".
+          rewrite H4. hred_r.
+          rewrite H4. hred_r.
+          rewrite co_co_members. ss. hred_r.
+          replace (Coqlib.align _ _) with 8%Z by et.
+          rewrite cast_ptrofs. hred_r.
+
+          iApply isim_ccallU_store; ss; oauto.
+          iSplitL "INV hd_point_key hd_ofs".
+          { iFrame. iExists _. iFrame.
+            iPureIntro. split; ss. exists 1. ss. }
+          iIntros (st_src10 st_tgt10) "[INV [hd_point_key hd_ofs]]".
+
+          hred_r. unhide. remove_tau.
+          rewrite hd_hdl_is_point. hred_r.
+          rewrite new_cast_ptr. hred_r.
+          iApply isim_ccallU_store; ss; oauto.
+          iSplitL "INV hd_hdl_point hd_hdl_ofs".
+          { iFrame. iExists _. iFrame. iPureIntro.
+            rewrite encode_val_length. ss. }
+          iIntros (st_src11 st_tgt11) "[INV [hd_hdl_point hd_hdl_ofs]]".
+
+          hred_r. remove_tau. hred_l. iApply isim_choose_src.
+          iExists _. iApply isim_ret.
+          iFrame. iSplit; ss. iSplit; ss.
+          iCombine "new_point_item new_point_key" as "new_point".
+          iCombine "hd_point_item hd_point_key" as "hd_point".
+          iPoseProof (points_to_collect with "new_point") as "new_point".
+          iPoseProof (points_to_collect with "hd_point") as "hd_point".
+
+          iPoseProof ((offset_slide _ _ _ _ _ (Ptrofs.repr (-8)%Z)) with "hd_ofs") as "hd_ofs".
+          replace (Val.addl (Val.addl _ _) _) with (Val.addl hd (Vptrofs Ptrofs.zero)).
+          2:{ rewrite Val.addl_assoc. ss. }
+          replace (Ptrofs.add (Ptrofs.add _ _) _) with Ptrofs.zero.
+          2:{ rewrite Ptrofs.add_assoc. ss. }
+          replace (Val.addl hd (Vptrofs Ptrofs.zero)) with hd by admit "capture should be add_null_r".
+
+          iExists _,_,_,_,_,_,_,_. iFrame.
+          iSplit; ss. unfold vlist_add.
+          destruct Val.eq; ss; cycle 1.
+          { destruct (Int.eq at_tail Int.zero) eqn: E; clarify.
+            apply Int.same_if_eq in E. clarify. }
+          { iExists Ptrofs.zero,i_hd',_,_. iFrame. rewrite Ptrofs.xor_zero_l.
+            iFrame. iSplit; ss.
+            unfold ptr_equiv. 
+            iDestruct "end_equiv" as "[%|[B|C]]".
+            { iPoseProof (capture_dup with "hd_addr") as "[hd_addr hd_addr']".
+              iPoseProof (capture_dup with "hd_addr'") as "[hd_addr' hd_addr'']".
+              iPoseProof (capture_pointto_comm with "hd_addr'") as "comm".
+              iPoseProof (capture_offset_comm with "hd_addr''") as "comm'".
+              iPoseProof ("comm" with "hd_point") as "hd_point".
+              iPoseProof ("comm'" with "hd_ofs") as "hd_ofs".
+              iExists _,Ptrofs.zero,_,_. iFrame.
+              rewrite Ptrofs.xor_zero. iFrame. 
+              clarify. iSplit; ss. iSplit; ss.
+              iRight. iRight. iExists _. iSplit; ss. iExists _. iFrame. }
+            { iDestruct "B" as (i0) "[% REL]".
+              iDestruct "REL" as (m) "REL".
+              iCombine "hd_point REL" as "hd".
+              iPoseProof (replace_meta_to_alive with "hd") as "[hd_point REL]".
+              iCombine "hd_addr REL" as "hd_addr".
+              iPoseProof (capture_unique with "hd_addr") as "%".
+              clarify.
+              iDestruct "hd_addr" as "[hd_addr _]".
+              iExists _,Ptrofs.zero,_,_. iFrame.
+              iPoseProof (capture_dup with "hd_addr") as "[hd_addr hd_addr']".
+              iPoseProof (capture_dup with "hd_addr'") as "[hd_addr' hd_addr'']".
+              iPoseProof (capture_pointto_comm with "hd_addr'") as "comm".
+              iPoseProof (capture_offset_comm with "hd_addr''") as "comm'".
+              iPoseProof ("comm" with "hd_point") as "hd_point".
+              iPoseProof ("comm'" with "hd_ofs") as "hd_ofs".
+              iFrame. 
+              rewrite Ptrofs.xor_zero. iFrame.
+              iSplit; ss. iSplit; ss. iLeft. ss. }
+            { iDestruct "C" as (i0) "[% REL]".
+              iDestruct "REL" as (m) "REL". clarify.
+              iPoseProof (capture_dup with "hd_addr") as "[hd_addr hd_addr']".
+              iPoseProof (capture_dup with "hd_addr'") as "[hd_addr' hd_addr'']".
+              iPoseProof (capture_pointto_comm with "hd_addr'") as "comm".
+              iPoseProof (capture_offset_comm with "hd_addr''") as "comm'".
+              iPoseProof ("comm" with "hd_point") as "hd_point".
+              iPoseProof ("comm'" with "hd_ofs") as "hd_ofs".
+              iExists _,Ptrofs.zero,_,_. iFrame.
+              rewrite Ptrofs.xor_zero. iFrame.
+              iSplit; ss. iSplit; ss. iRight. iRight. 
+              assert (i0 = i_hd') by admit "capture for int".
+              clarify. iExists _. iSplit; ss. iExists _. iFrame. } }
+        * destruct v; try solve [iDestruct "LIST" as "%"; clarify].
+          iDestruct "LIST" as (i_hd i_next_next m_hd' m_next)
+            "[[[[% hd_addr'] next_ofs] next_point] LIST]".
+          rename H4 into m_next_size.
+
+          iPoseProof ((offset_slide _ _ _ _ _ (Ptrofs.repr (-8)%Z)) with "new_ofs") as "new_ofs".
+          replace (Val.addl (Val.addl _ _) _) with p_new.
+          2:{ rewrite Val.addl_assoc. ss. }
+          replace (Ptrofs.add (Ptrofs.add _ _) _) with Ptrofs.zero.
+          2:{ rewrite Ptrofs.add_assoc. ss. }
+
+          iApply isim_ccallU_pure; et.
+          { eapply fn_has_spec_in_stb; et.
+            { eapply STBINCL. stb_tac. unfold xorStb.
+              unseal "stb". ss. }
+            { ss. instantiate (1:= (inl (_,_,_,_,_,_,_,_,_,_))).
+              ss. oauto. }
+            { ss. } }
+          { instantiate (1:=10). oauto. }
+
+          ss. iSplitL "INV new_ofs next_ofs".
+          { iSplit; ss. iSplit; ss. iSplitR "next_ofs"; ss. iFrame. ss. }
+          iIntros (st_src9 st_tgt9 ret_src0 ret_tgt0) "[INV [POST %]]".
+          iDestruct "POST" as (i_new i_next') "[[[[% new_ofs] next_ofs] new_addr] next_addr]".
+          rewrite H5. clear H5 H4.
+          iExists _. iSplit; ss.
+
+          hred_r. unhide. remove_tau.
+          rewrite hd_is_point. hred_r.
+          rewrite hd_is_point. hred_r.
+          rewrite co_co_members. ss. hred_r.
+          replace (Coqlib.align _ _) with 8%Z.
+          rewrite cast_ptrofs. hred_r.
+
+          iApply isim_ccallU_store; ss; oauto.
+          iSplitL "INV hd_point_key hd_ofs".
+          { iFrame. iExists _. iFrame. iPureIntro. split; ss. exists 1. ss. }
+          iIntros (st_src10 st_tgt10) "[INV [hd_point_key hd_ofs]]".
+
+          hred_r. unhide. remove_tau.
+          rewrite hd_hdl_is_point. hred_r.
+          rewrite new_cast_ptr. hred_r.
+
+          iApply isim_ccallU_store; ss; oauto.
+          iSplitL "INV hd_hdl_point hd_hdl_ofs".
+          { iFrame. iExists _. iFrame. iPureIntro. split; ss.
+            rewrite encode_val_length. ss. }
+          iIntros (st_src11 st_tgt11) "[INV [hd_hdl_point hd_hdl_ofs]]".
+
+          hred_r. remove_tau. 2: ss. hred_l. iApply isim_choose_src.
+          iExists _. iApply isim_ret. iSplit; ss. iSplit; ss. iSplit; ss.
+          iExists _,_,_,_,_,_,_,_. iFrame.
+          iSplit; ss.
+          unfold vlist_add.
+          destruct Val.eq; cycle 1.
+          { destruct (Int.eq at_tail Int.zero) eqn: E; clarify.
+            apply Int.same_if_eq in E. clarify. }
+
+
+          iCombine "new_point_item new_point_key" as "new_point".
+          iCombine "hd_point_item hd_point_key" as "hd_point".
+          iPoseProof (points_to_collect with "new_point") as "new_point".
+          iPoseProof (points_to_collect with "hd_point") as "hd_point".
+          iCombine "hd_point hd_addr'" as "hd".
+          iPoseProof (replace_meta_to_alive with "hd") as "[hd_point hd_addr']".
+          iCombine "hd_addr hd_addr'" as "hd_addr".
+          iPoseProof (capture_unique with "hd_addr") as "%".
+          clarify.
+          iDestruct "hd_addr" as "[_ hd_addr]".
+          iPoseProof ((offset_slide _ _ _ _ _ (Ptrofs.repr (-8)%Z)) with "hd_ofs") as "hd_ofs".
+          replace (Val.addl (Val.addl _ _) _) with hd.
+          2:{ rewrite Val.addl_assoc. admit "captured val plus null". }
+          replace (Ptrofs.add (Ptrofs.add _ _) _) with Ptrofs.zero.
+          2:{ rewrite Ptrofs.add_assoc. ss. }
+
+          ss. iExists _,i_hd,_,_. iFrame.
+          rewrite Ptrofs.xor_zero_l. iFrame. iSplit; ss.
+          iPoseProof (capture_dup with "hd_addr") as "[hd_addr hd_addr']".
+          iPoseProof (capture_dup with "hd_addr'") as "[hd_addr' hd_addr'']".
+          iPoseProof (capture_pointto_comm with "hd_addr'") as "comm".
+          iPoseProof (capture_offset_comm with "hd_addr''") as "comm'".
+          iPoseProof ("comm" with "hd_point") as "hd_point".
+          iPoseProof ("comm'" with "hd_ofs") as "hd_ofs".
+          iExists _,_,_,_. iFrame. iSplit; ss.
+          replace i_next' with i_next by admit "captured int is equal".
+          iExists _,_,_,_. iFrame. iSplit; ss.
+          iPoseProof (capture_refl with "hd_addr") as "?".
+          iFrame.
+          
+    +
+
+          
+
+
+
+
+
+        
+
   Admitted.
 
   End SIMFUNS.
